VOQC/GreedyLayout.v
@@ -1,6 +1,7 @@
 Require Import QuantumLib.VectorStates.
 Require Import MappingGateSet.
 Require Import Layouts.
+Require Import ConnectivityGraph.
 
 Require Import FSets.FSetAVL.
 Require Import FSets.FSetFacts.
@@ -36,7 +37,7 @@ Fixpoint get_fresh_qubit (prefs : list nat) (alloc : FSet.t) :=
    in the returned layout. Note that the layout may change during mapping 
    (due to inserted swaps) so this strategy will not always choose the best 
    placement. *)
-Fixpoint build_layout {U dim} (l : gate_list (Map_Unitary U) dim) (alloc : FSet.t) (lay : layout) (q_ordering : option nat -> list nat) : FSet.t * layout:=
+Fixpoint build_layout {U dim} (l : gate_list (Map_Unitary U) dim) (alloc : FSet.t) (lay : layout) (q_ordering : option nat -> list nat) : FSet.t * layout :=
   match l with
   | [] => (alloc, lay)
   | App2 UMap_CNOT m n :: t => 
@@ -54,7 +55,8 @@ Fixpoint build_layout {U dim} (l : gate_list (Map_Unitary U) dim) (alloc : FSet.
           build_layout t alloc' lay' q_ordering
       | None, None =>
           let m_phys := get_fresh_qubit (q_ordering None) alloc in
-          let n_phys := get_fresh_qubit (q_ordering (Some m_phys)) alloc in
+          let n_phys := get_fresh_qubit (q_ordering (Some m_phys)) 
+                                        (FSet.add m_phys alloc) in
           let alloc' := FSet.add n_phys (FSet.add m_phys alloc) in
           let lay' := add (add lay m m_phys) n n_phys in
           build_layout t alloc' lay' q_ordering
@@ -64,14 +66,14 @@ Fixpoint build_layout {U dim} (l : gate_list (Map_Unitary U) dim) (alloc : FSet.
 
 (** Choose a physical qubit for any unallocated logical qubits. n is the number
     of physical qubits available. *)
-Fixpoint extend_layout (n : nat) (alloc : FSet.t) (lay : layout) (q_ordering : option nat -> list nat)  :=
+Fixpoint extend_layout (n : nat) (alloc : FSet.t) (lay : layout) (prefs: list nat) :=
   match n with
   | O => lay
   | S n' => 
       match find_phys lay n' with 
-      | Some _ => extend_layout n' alloc lay q_ordering
-      | None => let m := get_fresh_qubit (q_ordering None) alloc in
-               extend_layout n' (FSet.add m alloc) (add lay n' m) q_ordering
+      | Some _ => extend_layout n' alloc lay prefs
+      | None => let m := get_fresh_qubit prefs alloc in
+               extend_layout n' (FSet.add m alloc) (add lay n' m) prefs
       end
   end.
 
@@ -79,7 +81,7 @@ Fixpoint extend_layout (n : nat) (alloc : FSet.t) (lay : layout) (q_ordering : o
    qubits available on the machine *)
 Definition greedy_layout {U dim} (l : gate_list (Map_Unitary U) dim) (n : nat) (q_ordering : option nat -> list nat) : layout :=
   let (alloc, lay) := build_layout l FSet.empty empty q_ordering in
-  extend_layout n alloc lay q_ordering.
+  extend_layout n alloc lay (q_ordering None).
 
 (** Proofs *)
 
@@ -195,25 +197,235 @@ Proof.
   apply H in Hadd. auto.
 Qed.
 
-(* TODO: move to CG *)
-Definition valid_q_ordering (q_ordering : option nat -> list nat) n :=
-  forall o x, x < n <-> List.In x (q_ordering o).
-
-(* Easy definition that satisfies the spec *)
-Fixpoint list_nats n := match n with O => [] | S n' => n' :: list_nats n' end.
-
-Lemma list_nats_is_valid_q_ordering : forall n, valid_q_ordering (fun _ => list_nats n) n.
+Lemma bounded_set_incomplete : forall (s : FSet.t) n,
+  FSet.cardinal s < n ->
+  (forall x, FSet.In x s -> x < n) ->
+  exists y, y < n /\ ~ FSet.In y s.
 Proof.
-  intros n o x.
-  induction n; simpl.
+  intros s n.
+  gen s.
+  induction n; intros s Hs1 Hs2.
+  lia.
+  remember (FSet.max_elt s) as o.
+  symmetry in Heqo.
+  destruct o.
+  - (* max_elt is Some *)
+    remember (FSet.remove e s) as s'.
+    assert (FSet.cardinal s' < n).
+    { rewrite <- FSetProps.remove_cardinal_1 with (x:=e) in Hs1.
+      subst. lia.
+      apply FSet.max_elt_1. auto. }
+    assert (forall x, FSet.In x s' -> x < n).
+    { intros x Hx.
+      subst s'.
+      assert (x <> e).
+      intro contra.
+      contradict Hx.
+      apply FSet.remove_1. auto.
+      bdestruct (x =? n).
+      subst.
+      apply FSet.remove_3 in Hx.
+      assert (Heqo':=Heqo).
+      eapply FSet.max_elt_2 in Heqo.
+      2: apply Hx.
+      apply FSet.max_elt_1 in Heqo'.
+      apply Hs2 in Heqo'.
+      lia.
+      apply FSet.remove_3 in Hx.
+      apply Hs2 in Hx. lia. }
+    specialize (IHn s' H H0). 
+    destruct IHn as [y [Hy1 Hy2]].
+    bdestruct (y =? e).
+    + (* y = e *)
+      subst.
+      exists n.
+      split; auto.
+      intro contra.
+      apply FSet.max_elt_2 with (x:=e) in contra; auto.
+    + (* y <> e *)
+      exists y.
+      split; auto.
+      intro contra.
+      contradict Hy2.
+      subst s'.
+      apply FSetProps.FM.remove_iff.
+      split; auto.
+  - (* max_elt is None *)
+    apply FSet.max_elt_3 in Heqo.
+    exists 0. split. lia.
+    apply FSetProps.empty_is_empty_1 in Heqo.
+    rewrite Heqo.
+    intro contra.
+    apply FSetFacts.empty_iff in contra.
+    auto.
+Qed.
+
+Fixpoint record_Somes (f : nat -> option nat) (n : nat) : FSet.t :=
+  match n with
+  | O => FSet.empty
+  | S n' => match f n' with
+           | None => record_Somes f n'
+           | Some x => FSet.add x (record_Somes f n')
+           end
+  end.
+
+Lemma record_Somes_size : forall f n x,
+  x < n -> f x = None ->
+  FSet.cardinal (record_Somes f n) < n.
+Proof.
+  assert (Haux: forall f n, FSet.cardinal (record_Somes f n) < S n).
+  { intros f n.
+    induction n; simpl.
+    rewrite FSetProps.empty_cardinal. lia.
+    destruct (f n).
+    destruct (FSetProps.In_dec n0 (record_Somes f n)).
+    rewrite FSetProps.add_cardinal_1 by assumption. lia.
+    rewrite FSetProps.add_cardinal_2 by assumption. lia.
+    lia. }
+  intros f n x H1 H2.
+  induction n; simpl in *.
   lia.
   bdestruct (x =? n).
   subst.
-  split; intro H; auto.
-  split; intro H0.
-  right. apply IHn. lia.
-  destruct H0 as [H0 | H0]; subst; try contradiction.
-  apply IHn in H0. lia.
+  rewrite H2.
+  apply Haux.
+  destruct (f n).
+  destruct (FSetProps.In_dec n0 (record_Somes f n)).
+  rewrite FSetProps.add_cardinal_1 by assumption. lia.
+  rewrite FSetProps.add_cardinal_2 by assumption. lia.
+  lia.
+Qed.
+
+Lemma record_Somes_find_phys_bounded : forall lay m n,
+  find_phys_bounded lay m -> 
+  forall x, FSet.In x (record_Somes (find_phys lay) n) -> x < m.
+Proof.
+  intros lay m n Hbnd x Hx.
+  induction n; simpl in *.
+  apply FSetFacts.empty_iff in Hx.
+  contradiction.
+  destruct (find_phys lay n) eqn:fl; auto.
+  apply Hbnd in fl.
+  apply FSetFacts.add_iff in Hx.
+  destruct Hx as [Hx | Hx]; auto.
+  lia.
+Qed.
+
+Lemma record_Somes_find_log_bounded : forall lay m n,
+  find_log_bounded lay m -> 
+  forall x, FSet.In x (record_Somes (find_log lay) n) -> x < m.
+Proof.
+  intros lay m n Hbnd x Hx.
+  induction n; simpl in *.
+  apply FSetFacts.empty_iff in Hx.
+  contradiction.
+  destruct (find_log lay n) eqn:fl; auto.
+  apply Hbnd in fl.
+  apply FSetFacts.add_iff in Hx.
+  destruct Hx as [Hx | Hx]; auto.
+  lia.
+Qed.
+
+Lemma record_Somes_correct : forall f n x,
+  FSet.In x (record_Somes f n) <-> exists y, y < n /\ f y = Some x.
+Proof.
+  intros f n x.  
+  induction n; simpl.
+  rewrite FSetFacts.empty_iff.
+  split; intro H; try easy.
+  destruct H as [? [? ?]]. lia.
+  split; intro H.
+  destruct (f n) eqn:fn.
+  apply FSetFacts.add_iff in H.
+  destruct H.
+  subst.
+  exists n. split; auto.
+  apply IHn in H as [y [? ?]].
+  exists y. split; auto.
+  apply IHn in H as [y [? ?]].
+  exists y. split; auto.
+  destruct H as [y [? ?]].
+  bdestruct (y =? n).
+  subst.
+  rewrite H0.
+  apply FSetFacts.add_iff.
+  left. auto.
+  destruct (f n) eqn:fn.
+  apply FSetFacts.add_iff.
+  right. apply IHn.
+  exists y. split. lia. auto.
+  apply IHn.
+  exists y. split. lia. auto.
+Qed.
+
+Lemma not_Some_implies_None : forall A (o : option A), ~ (exists x, o = Some x) -> o = None.
+Proof.
+  intros A o H.
+  destruct o; auto.
+  contradict H.
+  exists a. auto.
+Qed.
+
+Lemma find_phys_None_implies_find_log_None : forall lay n,
+  well_formed lay ->
+  find_log_bounded lay n ->
+  find_phys_bounded lay n ->
+  (exists x, x < n /\ find_phys lay x = None) ->
+  exists y, y < n /\ find_log lay y = None.
+Proof.
+  intros lay n WF Hlog Hphys [x [Hx1 Hx2]].
+  remember (record_Somes (find_phys lay) n) as s.
+  assert (FSet.cardinal s < n).
+  { subst s. eapply record_Somes_size. apply Hx1. auto. }
+  assert (forall x, FSet.In x s -> x < n).
+  { subst s. apply record_Somes_find_phys_bounded. auto. }
+  assert (exists y, y < n /\ ~ FSet.In y s).
+  { apply bounded_set_incomplete; auto. }
+  destruct H1 as [y [Hy1 Hy2]].
+  exists y.
+  split; auto.
+  subst s.
+  rewrite record_Somes_correct in Hy2.
+  apply not_Some_implies_None.
+  intro contra.
+  contradict Hy2.
+  destruct contra as [z Hz].
+  assert (z < n).
+  eapply Hlog. apply Hz.
+  apply WF in Hz.
+  exists z.
+  split; auto.
+Qed.
+
+Lemma find_log_None_implies_find_phys_None : forall lay n,
+  well_formed lay ->
+  find_log_bounded lay n ->
+  find_phys_bounded lay n ->
+  (exists x, x < n /\ find_log lay x = None) ->
+  exists y, y < n /\ find_phys lay y = None.
+Proof.
+  intros lay n WF Hlog Hphys [x [Hx1 Hx2]].
+  remember (record_Somes (find_log lay) n) as s.
+  assert (FSet.cardinal s < n).
+  { subst s. eapply record_Somes_size. apply Hx1. auto. }
+  assert (forall x, FSet.In x s -> x < n).
+  { subst s. apply record_Somes_find_log_bounded. auto. }
+  assert (exists y, y < n /\ ~ FSet.In y s).
+  { apply bounded_set_incomplete; auto. }
+  destruct H1 as [y [Hy1 Hy2]].
+  exists y.
+  split; auto.
+  subst s.
+  rewrite record_Somes_correct in Hy2.
+  apply not_Some_implies_None.
+  intro contra.
+  contradict Hy2.
+  destruct contra as [z Hz].
+  assert (z < n).
+  eapply Hphys. apply Hz.
+  apply WF in Hz.
+  exists z.
+  split; auto.
 Qed.
 
 Lemma find_phys_None_implies_alloc_incomplete : forall lay alloc q_ord n o,
@@ -223,14 +435,42 @@ Lemma find_phys_None_implies_alloc_incomplete : forall lay alloc q_ord n o,
   find_log_bounded lay n ->
   find_phys_bounded lay n ->
   (exists x, x < n /\ find_phys lay x = None) ->
+  (match o with Some y => find_log lay y <> None | _ => True end) ->
   exists x : FSet.elt, In x (q_ord o) /\ ~ FSet.In x alloc.
 Proof.
-  intros lay alloc q_ord n o Hqor WF Halloc Hlog Hphys [x [Hx1 Hx2]].
+  intros lay alloc q_ord n o Hqor WF Halloc Hlog Hphys [x [Hx1 Hx2]] Ho.
+  apply Classical_Pred_Type.not_all_not_ex.
+  intro contra.
+  assert (exists y, y < n /\ find_log lay y = None).
+  { eapply find_phys_None_implies_find_log_None; auto.
+    exists x. auto. }
+  destruct H as [y [Hy1 Hy2]].
+  specialize (contra y).
+  apply Classical_Prop.not_and_or in contra as [contra | contra].
+  contradict contra.                                                             
+  apply Hqor.
+  destruct o; auto.
+  split; auto.
+  intro contra.
+  subst. easy.
+  apply Classical_Prop.NNPP in contra.
+  apply Halloc in contra.
+  destruct contra as [z contra].
+  apply WF in contra.
+  rewrite contra in Hy2.
+  discriminate.
+Qed.
 
-
-(* stuck -- we probably need some kind of counting argument *)
-
-Admitted.
+Lemma valid_q_ordering_lt : forall q_ordering dim o,
+  valid_q_ordering q_ordering dim ->
+  forall x : nat, In x (q_ordering o) -> 
+  x < dim.
+Proof.
+  intros q_ordering dim o H1 x H2.
+  apply H1 in H2.
+  destruct o; auto.
+  destruct H2 as [? ?]; auto.
+Qed.
 
 Lemma build_layout_well_formed : forall U dim (l : gate_list (Map_Unitary U) dim) alloc lay q_ordering lay' alloc',
   well_formed lay ->
@@ -265,6 +505,7 @@ Proof.
     eapply find_phys_None_implies_alloc_incomplete.
     apply Hqor. apply WF. apply Halloc. apply Hlog. apply Hphys.
     exists n0. split; auto.
+    apply WF in fpn. rewrite fpn. easy.
     destruct contra as [p contra].
     apply WF in contra.
     rewrite fpn0 in contra.
@@ -273,10 +514,11 @@ Proof.
     apply find_log_bounded_add; auto.
     apply find_phys_bounded_add; auto.
     subst. apply get_fresh_qubit_lt.
-    intros. apply Hqor in H0. auto.
+    apply valid_q_ordering_lt. auto.
     eapply find_phys_None_implies_alloc_incomplete.
     apply Hqor. apply WF. apply Halloc. apply Hlog. apply Hphys.
     exists n0. split; auto.
+    apply WF in fpn. rewrite fpn. easy.
   - remember (get_fresh_qubit (q_ordering (Some n)) alloc) as x.
     apply IHl in H; auto; clear IHl.
     apply add_well_formed; auto.
@@ -287,6 +529,7 @@ Proof.
     eapply find_phys_None_implies_alloc_incomplete.
     apply Hqor. apply WF. apply Halloc. apply Hlog. apply Hphys.
     exists n. split; auto.
+    apply WF in fpn0. rewrite fpn0. easy.
     destruct contra as [p contra].
     apply WF in contra.
     rewrite fpn in contra.
@@ -295,113 +538,111 @@ Proof.
     apply find_log_bounded_add; auto.
     apply find_phys_bounded_add; auto.
     subst. apply get_fresh_qubit_lt.
-    intros. apply Hqor in H0. auto.
+    apply valid_q_ordering_lt. auto.
     eapply find_phys_None_implies_alloc_incomplete.
     apply Hqor. apply WF. apply Halloc. apply Hlog. apply Hphys.
     exists n. split; auto.
+    apply WF in fpn0. rewrite fpn0. easy.
   - remember (get_fresh_qubit (q_ordering None) alloc) as x.
     remember (get_fresh_qubit (q_ordering (Some x)) (FSet.add x alloc)) as y.
+    assert (WF' : well_formed (add lay n x)).
+    { apply add_well_formed; auto.
+      intros [contra | contra].
+      apply Halloc in contra.
+      contradict contra.
+      subst x. apply get_fresh_qubit_not_In_alloc.
+      eapply find_phys_None_implies_alloc_incomplete.
+      apply Hqor. apply WF. apply Halloc. apply Hlog. apply Hphys.
+      exists n. split; auto. easy.
+      destruct contra as [p contra].
+      apply WF in contra.
+      rewrite fpn in contra.
+      inversion contra. }
+    assert (Halloc' : alloc_records_allocated_phys_qubits (add lay n x) (FSet.add x alloc)).
+    { apply alloc_records_allocated_phys_qubits_add; auto. }
+    assert (x < dim).
+    { subst x. apply get_fresh_qubit_lt.
+      intros. apply Hqor in H0. auto.
+      eapply find_phys_None_implies_alloc_incomplete.
+      apply Hqor. apply WF. apply Halloc. apply Hlog. apply Hphys.
+      exists n. split; auto. easy. }
+    assert (y < dim).
+    { subst y.  apply get_fresh_qubit_lt.
+      apply valid_q_ordering_lt. auto.
+      eapply find_phys_None_implies_alloc_incomplete.
+      apply Hqor. apply WF'. apply Halloc'.
+      apply find_log_bounded_add; auto.
+      apply find_phys_bounded_add; auto.
+      exists n0. split; auto.
+      rewrite find_phys_add_neq; auto.
+      rewrite find_log_add_eq. easy. }
     apply IHl in H; auto; clear IHl.
     apply add_well_formed; auto.
-    apply add_well_formed; auto.
     intros [contra | contra].
-    apply Halloc in contra.
+    apply Halloc' in contra.
     contradict contra.
-    subst. apply get_fresh_qubit_not_In_alloc.
+    subst y. apply get_fresh_qubit_not_In_alloc.
     eapply find_phys_None_implies_alloc_incomplete.
-    apply Hqor. apply WF. apply Halloc. apply Hlog. apply Hphys.
-    exists n. split; auto.
+    apply Hqor. 
+    apply WF'.
+    apply Halloc'.
+    apply find_log_bounded_add; auto.
+    apply find_phys_bounded_add; auto.
+    exists n0. split; auto.
+    rewrite find_phys_add_neq; auto.
+    rewrite find_log_add_eq. easy.
     destruct contra as [p contra].
-    apply WF in contra.
-    rewrite fpn in contra.
-    inversion contra. 
-    apply not_In_add; auto.
-     admit. (* y <> x ; y is not in (FSet.add x alloc) *)
-    intros [contra | contra].
-    apply Halloc in contra.
-    contradict contra.
-    subst. apply get_fresh_qubit_not_In_alloc.
-    eapply find_phys_None_implies_alloc_incomplete.
-    apply Hqor. apply WF. apply Halloc. apply Hlog. apply Hphys.
-    exists n. split; auto.
-    destruct contra as [p contra].
-    apply WF in contra.
+    apply WF' in contra.
+    rewrite find_phys_add_neq in contra; auto.
     rewrite fpn0 in contra.
     inversion contra.
     apply alloc_records_allocated_phys_qubits_add; auto.
     rewrite find_phys_add_neq; auto.
-    apply alloc_records_allocated_phys_qubits_add; auto.
     apply find_log_bounded_add; auto.
     apply find_log_bounded_add; auto.
     apply find_phys_bounded_add; auto.
     apply find_phys_bounded_add; auto.
-    subst. apply get_fresh_qubit_lt.
-    intros. apply Hqor in H0. auto.
-    eapply find_phys_None_implies_alloc_incomplete.
-    apply Hqor. apply WF. apply Halloc. apply Hlog. apply Hphys.
-    exists n. split; auto.
-    subst. apply get_fresh_qubit_lt.
-    intros. apply Hqor in H0. auto.
-    eapply find_phys_None_implies_alloc_incomplete.
-    apply Hqor. apply WF. apply Halloc. apply Hlog. apply Hphys.
-    exists n. split; auto.
-Admitted.
+Qed.
 
-Lemma find_log_extend_layout1 : forall n alloc lay q_ordering p l,
-  alloc_records_allocated_phys_qubits lay alloc ->
-  find_log lay p = Some l ->
-  find_log (extend_layout n alloc lay q_ordering) p = Some l.
-Proof.
-  intros n alloc lay q_ordering p l.
-  gen alloc lay.
-  induction n; intros alloc lay H1 H2; simpl; auto.
-  destruct (find_phys lay n) eqn:fp.
-  auto.
-  apply IHn.
-  apply alloc_records_allocated_phys_qubits_add; auto.
-  rewrite find_log_add_neq; auto.
-  (* "get_default q_ordering alloc" is not in alloc, but p is *)
-Admitted.
-
-Lemma find_log_extend_layout2 : forall m n alloc lay q_ordering p,
-  (p < n)%nat ->
+Lemma extend_layout_well_formed : forall dim n alloc lay q_ordering,
   well_formed lay ->
   alloc_records_allocated_phys_qubits lay alloc ->
-  find_log lay p = None ->
-  exists l, find_log (extend_layout n alloc lay q_ordering) p = Some l /\ (l < m)%nat.
+  find_log_bounded lay dim ->
+  find_phys_bounded lay dim ->
+  valid_q_ordering q_ordering dim ->
+  n <= dim ->
+  well_formed (extend_layout n alloc lay (q_ordering None)).
 Proof.
-  intros m n alloc lay q_ordering p Hp.
+  intros dim n alloc lay q_ordering ? ? ? ? Hqor.
   gen alloc lay.
-  induction n; intros alloc lay H1 H2 H3; simpl; auto.
-lia.
-
-(*
-bdestruct (p =? n).
-subst. clear IHn.
-
-destruct (find_phys lay n) eqn:fp.
-
-  exists (get_default q_ordering alloc).
+  induction n; intros alloc lay WF Halloc  Hlog Hphys Hn; simpl; auto.
+  destruct (find_phys lay n) eqn:fp.
+  apply IHn; auto. lia.
+  apply IHn.
+  apply add_well_formed; auto.
+  apply Classical_Prop.and_not_or.
   split.
-  erewrite find_phys_extend_layout1.
-  reflexivity.
+  intro contra.
+  apply Halloc in contra.
+  contradict contra.
+  apply get_fresh_qubit_not_In_alloc.
+  eapply find_phys_None_implies_alloc_incomplete.
+  apply Hqor. apply WF. apply Halloc. apply Hlog. apply Hphys.
+  exists n. split; auto. easy.
+  intros [p contra].
+  apply WF in contra.
+  rewrite fp in contra.
+  inversion contra.
   apply alloc_records_allocated_phys_qubits_add; auto.
-  apply find_phys_add_eq.
-
-
-admit.
-
-
-destruct (find_phys lay n) eqn:fp.
-
-apply IHn; auto. lia.
-
-apply IHn. lia.
-  apply alloc_records_allocated_phys_qubits_add; auto.
-  rewrite find_log_add_neq; auto.
-*)
-
- Admitted.
+  apply find_log_bounded_add; auto.
+  apply find_phys_bounded_add; auto.
+  apply get_fresh_qubit_lt.
+  apply Hqor.
+  eapply find_phys_None_implies_alloc_incomplete.
+  apply Hqor. apply WF. apply Halloc. apply Hlog. apply Hphys.
+  exists n. split; auto. easy.
+  lia.
+Qed.
 
 Lemma find_phys_extend_layout1 : forall n alloc lay q_ordering l p,
   alloc_records_allocated_phys_qubits lay alloc ->
@@ -420,17 +661,20 @@ Proof.
   rewrite H2 in fp. inversion fp.
 Qed.
 
-Lemma find_phys_extend_layout2 : forall m n alloc lay q_ordering l,
+Lemma find_phys_extend_layout2 : forall dim n alloc lay q_ordering l,
   (l < n)%nat ->
   well_formed lay ->
   alloc_records_allocated_phys_qubits lay alloc ->
-  valid_q_ordering q_ordering m ->
+  find_log_bounded lay dim ->
+  find_phys_bounded lay dim ->
+  valid_q_ordering q_ordering dim ->
+  n <= dim ->
   find_phys lay l = None ->
-  exists p, find_phys (extend_layout n alloc lay q_ordering) l = Some p /\ (p < m)%nat.
+  exists p, find_phys (extend_layout n alloc lay (q_ordering None)) l = Some p /\ (p < dim)%nat.
 Proof.
-  intros m n alloc lay q_ordering l Hl ? ? Hqor.
+  intros dim n alloc lay q_ordering l Hl ? ? ? ? Hqor.
   gen alloc lay.
-  induction n; intros alloc lay WF Halloc H; simpl; auto.
+  induction n; intros alloc lay WF Halloc Hlog Hphys Hn H; simpl; auto.
   lia.
   bdestruct (l =? n).
   subst. clear IHn.
@@ -441,44 +685,126 @@ Proof.
   reflexivity.
   apply alloc_records_allocated_phys_qubits_add; auto.
   apply find_phys_add_eq.
-  apply get_fresh_qubit_lt.
-  intros. apply Hqor in H0. auto.
+  apply get_fresh_qubit_lt. apply Hqor.
   eapply find_phys_None_implies_alloc_incomplete.
-  apply Hqor. apply WF. apply Halloc. (*apply Hlog. apply Hphys.
-  exists n. split; auto.
-  admit. (*  (get_default q_ordering alloc < m)%nat *)
+  apply Hqor. apply WF. apply Halloc. apply Hlog. apply Hphys.
+  exists n. split; auto. easy.
+  destruct (find_phys lay n) eqn:fp.
+  apply IHn; auto. lia. lia.
+  apply IHn. lia.
+  apply add_well_formed; auto.
+  intros [contra | contra].
+  apply Halloc in contra.
+  contradict contra.
+  apply get_fresh_qubit_not_In_alloc.
+  eapply find_phys_None_implies_alloc_incomplete.
+  apply Hqor. apply WF. apply Halloc. apply Hlog. apply Hphys.
+  exists n. split; auto. easy. 
+  destruct contra as [? contra].
+  apply WF in contra. rewrite fp in contra. inversion contra.
+  apply alloc_records_allocated_phys_qubits_add; auto.
+  apply find_log_bounded_add; auto.
+  apply find_phys_bounded_add; auto.
+  apply get_fresh_qubit_lt.
+  apply Hqor.
+  eapply find_phys_None_implies_alloc_incomplete.
+  apply Hqor. apply WF. apply Halloc. apply Hlog. apply Hphys.
+  exists n. split; auto. easy.
+  lia.
+  rewrite find_phys_add_neq; auto.
+Qed.
+
+Lemma find_log_extend_layout_bounded : forall dim n alloc lay prefs,
+  n <= dim ->
+  find_log_bounded lay dim ->
+  find_log_bounded (extend_layout n alloc lay prefs) dim.
+Proof.
+  intros dim n alloc lay prefs Hn.
+  gen alloc lay.
+  induction n; intros alloc lay Hlog; simpl; auto.
   destruct (find_phys lay n) eqn:fp.
   apply IHn; auto. lia.
   apply IHn. lia.
-  apply alloc_records_allocated_phys_qubits_add; auto.
-  rewrite find_phys_add_neq; auto.*)
-Admitted.
+  apply find_log_bounded_add; auto.
+Qed.
 
-Lemma extend_layout_well_formed : forall n alloc lay q_ordering,
+Lemma find_phys_extend_layout_bounded : forall dim n alloc lay q_ordering,
   well_formed lay ->
   alloc_records_allocated_phys_qubits lay alloc ->
-  well_formed (extend_layout n alloc lay q_ordering).
+  find_log_bounded lay dim ->
+  find_phys_bounded lay dim ->
+  valid_q_ordering q_ordering dim ->
+  n <= dim ->
+  find_phys_bounded (extend_layout n alloc lay (q_ordering None)) dim.
 Proof.
-  intros n alloc lay q_ordering.
+  intros dim n alloc lay q_ordering ? ? ? ? Hqor Hn.
   gen alloc lay.
-  induction n; intros alloc lay H1 H2; simpl; auto.
+  induction n; intros alloc lay WF Halloc Hlog Hphys; simpl; auto.
   destruct (find_phys lay n) eqn:fp.
-  apply IHn; auto.
-  apply IHn.
+  apply IHn; auto. lia.
+  apply IHn. lia.
   apply add_well_formed; auto.
-  apply Classical_Prop.and_not_or.
-  split.
-  intro contra.
-  apply H2 in contra.
-  assert (~ (FSet.In (get_fresh_qubit (q_ordering None) alloc) alloc)).
-  admit.
-  contradiction.
-  intros [p contra].
-  apply H1 in contra.
-  rewrite fp in contra.
-  inversion contra.
+  intros [contra | contra].
+  apply Halloc in contra.
+  contradict contra.
+  apply get_fresh_qubit_not_In_alloc.
+  eapply find_phys_None_implies_alloc_incomplete.
+  apply Hqor. apply WF. apply Halloc. apply Hlog. apply Hphys.
+  exists n. split; auto. easy. 
+  destruct contra as [? contra].
+  apply WF in contra. rewrite fp in contra. inversion contra.
   apply alloc_records_allocated_phys_qubits_add; auto.
-Admitted.
+  apply find_log_bounded_add; auto.
+  apply find_phys_bounded_add; auto.
+  apply get_fresh_qubit_lt.
+  apply Hqor.
+  eapply find_phys_None_implies_alloc_incomplete.
+  apply Hqor. apply WF. apply Halloc. apply Hlog. apply Hphys.
+  exists n. split; auto. easy.
+Qed.
+
+Lemma find_log_extend_layout : forall dim alloc lay q_ordering p,
+  (p < dim)%nat ->
+  well_formed lay ->
+  alloc_records_allocated_phys_qubits lay alloc ->
+  find_log_bounded lay dim ->
+  find_phys_bounded lay dim ->
+  valid_q_ordering q_ordering dim ->
+  exists l, find_log (extend_layout dim alloc lay (q_ordering None)) p = Some l /\ (l < dim)%nat.
+Proof.
+  intros dim alloc lay q_ordering p Hp WF Halloc Hlog Hphys Hqor.
+  remember (extend_layout dim alloc lay (q_ordering None)) as elay.
+  apply Classical_Pred_Type.not_all_not_ex.
+  intro Hcontra.
+  assert (contra: find_log elay p = None).
+  { apply not_Some_implies_None.
+    intros [? contra].
+    assert (x < dim).
+    eapply find_log_extend_layout_bounded with (n:=dim). 
+    lia. apply Hlog. subst elay. apply contra.
+    specialize (Hcontra x).
+    apply Classical_Prop.not_and_or in Hcontra as [? | ?]; auto. }
+  clear Hcontra.
+  assert (H: exists p, p < dim /\ find_log elay p = None).
+  { exists p. auto. }
+  clear contra.
+  apply find_log_None_implies_find_phys_None in H.
+  destruct H as [? [? H]].
+  destruct (find_phys lay x) eqn:fp.
+  eapply find_phys_extend_layout1 with (n:=dim) (q_ordering:=q_ordering None) in fp; auto.
+  2: apply Halloc.
+  rewrite <- Heqelay in fp.
+  rewrite H in fp. inversion fp.
+  eapply find_phys_extend_layout2 with (n:=dim) (dim:=dim) in fp; auto.
+  2: apply Halloc.
+  2: apply Hqor.
+  destruct fp as [? [fp ?]].
+  rewrite <- Heqelay in fp.
+  rewrite H in fp. inversion fp.
+  subst. apply extend_layout_well_formed with (dim:=dim); auto.
+  subst. apply find_log_extend_layout_bounded; auto.
+  subst. apply find_phys_extend_layout_bounded; auto.
+Qed.
 
 Lemma extend_layout_bijective : forall n alloc lay q_ordering,
   well_formed lay ->
@@ -486,11 +812,11 @@ Lemma extend_layout_bijective : forall n alloc lay q_ordering,
   find_log_bounded lay n ->
   find_phys_bounded lay n ->
   valid_q_ordering q_ordering n ->
-  layout_bijective n (extend_layout n alloc lay q_ordering).
+  layout_bijective n (extend_layout n alloc lay (q_ordering None)).
 Proof.
   intros n alloc lay q_ordering WF H1 H2 H3 H4.
   split; [|split].
-  - apply extend_layout_well_formed; auto.
+  - apply extend_layout_well_formed with (dim:=n); auto.
   - intros l Hl.
     destruct (find_phys lay l) eqn:fp.
     exists n0.
@@ -499,16 +825,9 @@ Proof.
     apply H3 in fp. auto.
     apply find_phys_extend_layout2; auto.
   - intros p Hp.
-    destruct (find_log lay p) eqn:fl.
-    exists n0.
-    split.
-    apply find_log_extend_layout1; auto.
-    apply H2 in fl. auto.
-    apply find_log_extend_layout2; auto.
+    apply find_log_extend_layout; auto.
 Qed.
 
-(** dim is the number of qubits used in the program l and n is the number of
-   qubits available on the machine *)
 Lemma greedy_layout_bijective : forall U dim (l : gate_list (Map_Unitary U) dim) q_ordering,
   uc_well_typed_l l ->
   valid_q_ordering q_ordering dim ->
